lockservice: support dynamically reserving lock names

src/program_proof/lockservice/proof.v
@@ -1,6 +1,6 @@
 From Coq.Structures Require Import OrdersTac.
 From stdpp Require Import gmap.
-From iris.algebra Require Import numbers.
+From iris.algebra Require Import numbers coPset gset.
 From iris.program_logic Require Export weakestpre.
 From Perennial.goose_lang Require Import prelude.
 From Perennial.goose_lang Require Import ffi.disk_prelude.
@@ -13,96 +13,176 @@ From Perennial.Helpers Require Import NamedProps.
 From Perennial.Helpers Require Import ModArith.
 From Perennial.program_proof.lockservice Require Import lockservice fmcounter_map rpc common_proof nondet.
 
+Record lockserviceGN := LockserviceGN {
+  ls_rpcGN : RPC_GS;
+  ls_locksAllocGN : gname;
+  ls_locksMapDomGN : gname;
+}.
+
+Class lockserviceG Σ := LockserviceG {
+  ls_rpcG :> rpcG Σ u64; (* RPC layer ghost state *)
+  ls_locksAllocG :> mapG Σ u64 bool; (* [ls_locksAllocGN]: tracks with locks *logically* exist; true=exists *)
+  ls_locksMapDomG :> ghost_varG Σ (gset u64); (* [ls_mapDomGN]: Tracking the set of locks that *physically* exist *)
+}.
+
+Definition lockserviceN := nroot .@ "lockservice".
+Definition lockserviceInvN := nroot .@ "lockservice" .@ "inv".
+Definition locknameN (lockname : u64) := lockserviceN .@ "lock" .@ lockname.
+
 Section lockservice_proof.
-Context `{!heapG Σ}.
+Context `{!heapG Σ, !lockserviceG Σ}.
+Context {Ps : u64 -> iProp Σ}. (* Per-lock invariant *)
 
-Implicit Types s : Slice.t.
-Implicit Types (stk:stuckness) (E: coPset).
+Implicit Types (γ : lockserviceGN).
 
-Definition locknameN (lockname : u64) := nroot .@ "lock" .@ lockname.
+(** A token for being allowed to allocate a lock name. *)
+Definition lockservice_alloc_token γ (ln:u64) : iProp Σ :=
+  ln [[ γ.(ls_locksAllocGN) ]]↦ false.
 
-  Context `{!rpcG Σ u64}.
-  Context `{!mapG Σ (u64*u64) unit}.
-  Context `{Ps : u64 -> iProp Σ}.
-
-  Parameter validLocknames : gmap u64 unit.
-
+(** Witness showing that this lock exists *)
+Definition lockservice_is_lock γ (ln:u64) : iProp Σ :=
+  ln [[ γ.(ls_locksAllocGN) ]]↦ro true.
 
 Definition TryLock_Post : u64 -> u64 -> iProp Σ := λ args reply, (⌜reply = 0⌝ ∨ ⌜reply = 1⌝ ∗ (Ps args))%I.
-Definition TryLock_Pre : u64 -> iProp Σ := λ args, ⌜is_Some (validLocknames !! args)⌝%I.
+Definition TryLock_Pre γ : u64 -> iProp Σ := (λ args, lockservice_is_lock γ args)%I.
 
 Definition Unlock_Post : u64 -> u64 -> iProp Σ := λ args reply, True %I.
-Definition Unlock_Pre : u64 -> iProp Σ := λ args, (⌜is_Some (validLocknames !! args)⌝ ∗ (Ps args))%I.
+Definition Unlock_Pre γ : u64 -> iProp Σ := (λ args, lockservice_is_lock γ args ∗ (Ps args))%I.
 
-Definition LockServer_own_core (srv:loc) : iProp Σ :=
-  ∃ (locks_ptr:loc) (locksM:gmap u64 bool),
-  "HlocksOwn" ∷ srv ↦[LockServer.S :: "locks"] #locks_ptr
-∗ ("Hlockeds" ∷ [∗ map] ln ↦ locked ; _ ∈ locksM ; validLocknames, (⌜locked=true⌝ ∨ (Ps ln)))
-∗ "HlocksMap" ∷ is_map (locks_ptr) locksM
+(** Lockserver invariant (maintained even when the Mutex is held) *)
+Definition Lockserver_inv γ : iProp Σ :=
+  ∃ (locksAlloc: gmap u64 bool) (locksMapDom:gset u64),
+    "Hdom" ∷ ghost_var γ.(ls_locksMapDomGN) (1/2) locksMapDom ∗ (* we know the lock domain *)
+    "Hlocks" ∷ map_ctx γ.(ls_locksAllocGN) 1 locksAlloc ∗ (* we own the logical lock tracking *)
+    "HlocksEx" ∷ ⌜locksMapDom ⊆ dom (gset _) locksAlloc⌝ ∗ (* all physically-existing locks exist logically *)
+    "HlocksNew" ∷ [∗ map] ln ↦ ex ∈ locksAlloc,
+      (* all logically-existing locks either exist physically or have their invariant here *)
+      (⌜ex = false ∨ ln ∈ locksMapDom⌝ ∨ Ps ln)
 .
 
-Definition is_lockserver := is_server (Server_own_core:=LockServer_own_core).
+(** Lockserver mutex invariant *)
+Definition LockServer_own_core γ (srv:loc) : iProp Σ :=
+  ∃ (locks_ptr:loc) (locksM:gmap u64 bool),
+    "HlocksOwn" ∷ srv ↦[LockServer.S :: "locks"] #locks_ptr ∗ (* we own the "locks" field *)
+    "Hmap" ∷ is_map (locks_ptr) locksM ∗ (* we control the physical map *)
+    "HmapDom" ∷ ghost_var γ.(ls_locksMapDomGN) (1/2) (dom (gset _) locksM) ∗ (* the physical domain ghost variable matches the physical map *)
+    "Hlockeds" ∷ [∗ map] ln ↦ locked ∈ locksM, (⌜locked=true⌝ ∨ (Ps ln)) (* we own the invariants of all not-held locks *)
+.
 
-Lemma tryLock_core_spec (srv:loc) (tryLockArgs:u64) :
+Definition is_lockserver (srv:loc) γ : iProp Σ :=
+  "#Hinv" ∷ inv lockserviceInvN (Lockserver_inv γ) ∗
+  "#Hmutex" ∷ is_server (Server_own_core:=LockServer_own_core γ) srv γ.(ls_rpcGN).
+
+(** Allocate a new lock in the lockservice, given the corresponding token
+and the lock invariant. *)
+Lemma lockservice_alloc_lock γ (srv:loc) ln E :
+  ↑lockserviceN ⊆ E →
+  is_lockserver srv γ -∗
+  Ps ln -∗
+  lockservice_alloc_token γ ln ={E}=∗ lockservice_is_lock γ ln.
+Proof.
+  iIntros (?) "Hserver HP Htok". iNamed "Hserver".
+  iInv "Hinv" as "Hlockinv".
+  (* FIXME: looks like iNamed does not handle the ▷ here *)
+  iDestruct "Hlockinv" as (locksAlloc locksMapDom) "(>Hdom & >Hlocks & >HlocksEx & HlocksNew)".
+  iDestruct (map_valid with "Hlocks Htok") as %Hlookup.
+  iMod (map_update ln false true with "Hlocks Htok") as "[Hlocks Htok]".
+  iMod (map_freeze with "Hlocks Htok") as "[Hlocks $]".
+  iModIntro. iSplitL; last done. iNext.
+  iExists _, locksMapDom. iFrame. iSplit.
+  - iDestruct "HlocksEx" as %HlocksEx. iPureIntro. set_solver.
+  - iApply (big_sepM_insert_override_2 with "HlocksNew"); first done.
+    iIntros "_". eauto.
+Qed.
+
+Lemma tryLock_core_spec γ (srv:loc) (ln:u64) :
+inv lockserviceInvN (Lockserver_inv γ) -∗
 {{{ 
-     LockServer_own_core srv ∗ TryLock_Pre tryLockArgs
+     LockServer_own_core γ srv ∗ TryLock_Pre γ ln
 }}}
-  LockServer__tryLock_core #srv #tryLockArgs
+  LockServer__tryLock_core #srv #ln
 {{{
-   v, RET v; LockServer_own_core srv
-      ∗ (∃b:u64, ⌜v = #b⌝ ∗ TryLock_Post tryLockArgs b)
+   v, RET v; LockServer_own_core γ srv
+      ∗ (∃b:u64, ⌜v = #b⌝ ∗ TryLock_Post ln b)
 }}}.
 Proof.
-  iIntros (Φ) "[Hlsown Hpre] Hpost".
+  iIntros "#Hinv" (Φ) "!# [Hlsown #Hpre] Hpost".
   wp_lam.
   wp_let.
   iNamed "Hlsown".
   wp_loadField.
-  wp_apply (wp_MapGet with "HlocksMap"); eauto.
+  wp_apply (wp_MapGet with "Hmap"); eauto.
   iIntros (locked ok) "[% HlocksMap]".
-  iDestruct "Hpre" as %Hpre.
+  rewrite /TryLock_Pre.
+  wp_pures.
   destruct locked.
-  + (* Lock already held by someone *)
+  - (* Lock already held by someone *)
     wp_pures.
     iApply "Hpost".
     iSplitR "".
     { iExists _, _; iFrame. }
     iExists _. iSplit; eauto; last by iLeft.
-  + wp_pures.
+  - wp_pures.
     wp_loadField.
     wp_apply (wp_MapInsert with "HlocksMap"); first eauto; iIntros "HlocksMap".
-    iDestruct (big_sepM2_dom with "Hlockeds") as %HlocksDom.
-    iDestruct (big_sepM2_delete _ _ _ tryLockArgs false () with "Hlockeds") as "[HP Hlockeds]".
-    {
-      rewrite /map_get in H.
-      assert (is_Some (locksM !! tryLockArgs)) as HLocknameInLocks.
-      { apply elem_of_dom. apply elem_of_dom in Hpre. rewrite HlocksDom. done. }
-      destruct HLocknameInLocks as [ x  HLocknameInLocks].
-      rewrite HLocknameInLocks in H.
-        by injection H as ->.
-    }
-    { by destruct Hpre as [ [] HLocknameValid]. }
-    iDestruct (big_sepM2_insert_delete _ _ _ tryLockArgs true () with "[$Hlockeds]") as "Hlockeds"; eauto.
-    iDestruct "HP" as "[%|HP]"; first discriminate.
-    wp_pures. iApply "Hpost".
+    destruct ok.
+    + (* Lock already existed. *)
+      apply map_get_true in H.
+      iDestruct (big_sepM_insert_acc with "Hlockeds") as "[HP Hlockeds]"; first done.
+      iDestruct "HP" as "[%|HP]"; first done.
+      iSpecialize ("Hlockeds" $! true with "[]"); first by eauto.
+      
+      wp_pures. iApply "Hpost".
 
-    replace (<[tryLockArgs:=()]> validLocknames) with (validLocknames).
-    2:{ rewrite insert_id; eauto. by destruct Hpre as [ [] HLocknameValid]. }
+      rewrite /TryLock_Post.
+      iSplitR "HP"; last by eauto with iFrame.
 
-    iSplitR "HP".
-    { iExists _, _; iFrame. }
-    iExists _; iSplit; eauto.
-    iRight. by iFrame.
+      iExists _, _; iFrame.
+      replace (dom (gset u64) (<[ln:=true]> locksM)) with (dom (gset u64) locksM); first done.
+      rewrite dom_insert_L.
+      assert (ln ∈ dom (gset u64) locksM).
+      { apply elem_of_dom. eauto. }
+      set_solver.
+    + (* The lock did not exist yet, we have to "physically allocate" it. *)
+      apply map_get_false in H as [H _].
+      iApply fupd_wp.
+      iInv "Hinv" as (locksAlloc locksDom) "(>Hdom & >Hlocks & >HlocksEx & HlocksNew)".
+      iDestruct (ghost_var_agree with "HmapDom Hdom") as %<-.
+      iMod (ghost_var_update_halves ({[ ln ]} ∪ dom (gset _) locksM) with "HmapDom Hdom") as "[HmapDom Hdom]".
+      iDestruct (map_valid with "Hlocks Hpre") as %Halloc.
+      iDestruct (big_sepM_delete with "HlocksNew") as "[HP HlocksNew]"; first exact Halloc.
+      iDestruct "HP" as "[>HP|HP]".
+      { iDestruct "HP" as %[HP|HP%elem_of_dom]; first done. exfalso.
+        destruct HP as [? HP]. rewrite HP in H. done. }
+      iModIntro. iSplitL "HlocksNew HlocksEx Hlocks Hdom".
+      { iNext. iExists _, _. iFrame "Hdom Hlocks".
+        iSplit.
+        - iDestruct "HlocksEx" as %HlocksEx. iPureIntro.
+          assert (ln ∈ dom (gset _) locksAlloc). { apply elem_of_dom. eauto. }
+          set_solver.
+        - iApply (big_sepM_delete _ _ ln); first done. iSplitR.
+          { iLeft. iPureIntro. right. set_solver. }
+          iApply (big_sepM_mono with "HlocksNew").
+          intros ln' ? _. simpl. iIntros "[Hln'|Hln']"; last by eauto.
+          iLeft. iDestruct "Hln'" as %[?|Hln']; first by eauto.
+          iPureIntro. right. set_solver. }
+      iModIntro. wp_pures. iApply "Hpost".
+
+      rewrite /TryLock_Post.
+      iSplitR "HP"; last by eauto with iFrame.
+      iExists _, _. iFrame.
+      rewrite /typed_map.map_insert dom_insert_L. iFrame "HmapDom".
+      iApply big_sepM_insert; first done. iFrame "Hlockeds". eauto.
 Qed.
 
-Lemma unlock_core_spec (srv:loc) (unLockArgs:u64) :
+Lemma unlock_core_spec γ (srv:loc) (ln:u64) :
 {{{
-     LockServer_own_core srv ∗ Unlock_Pre unLockArgs
+     LockServer_own_core γ srv ∗ Unlock_Pre γ ln
 }}}
-  LockServer__unlock_core #srv #unLockArgs
+  LockServer__unlock_core #srv #ln
 {{{
-   v, RET v; LockServer_own_core srv
-      ∗ (∃b:u64, ⌜v = #b⌝ ∗ Unlock_Post unLockArgs b)
+   v, RET v; LockServer_own_core γ srv
+      ∗ (∃b:u64, ⌜v = #b⌝ ∗ Unlock_Post ln b)
 }}}.
 Proof.
   iIntros (Φ) "[Hlsown Hpre] Hpost".
@@ -110,90 +190,85 @@ Proof.
   wp_let.
   iNamed "Hlsown".
   wp_loadField.
-  wp_apply (wp_MapGet with "HlocksMap"); eauto.
+  wp_apply (wp_MapGet with "Hmap"); eauto.
   iIntros (locked ok) "[% HlocksMap]".
   destruct locked.
-  {
+  - (* Locks was previously held. *)
+    destruct ok; last first.
+    { (* Not already in domain? Impossible. *)
+      apply map_get_false in H as [_ H]. done. }
+    apply map_get_true in H.
     wp_pures.
     wp_loadField.
     wp_apply (wp_MapInsert with "HlocksMap"); eauto; iIntros "HlocksMap".
-    iDestruct "Hpre" as (Hpre) "HP".
-    iDestruct (big_sepM2_dom with "Hlockeds") as %HlocksDom.
-    iDestruct (big_sepM2_delete _ _ _ unLockArgs true () with "Hlockeds") as "[H_ Hlockeds]"; eauto.
-    {
-      rewrite /map_get in H.
-      assert (is_Some (locksM !! unLockArgs)) as HLocknameInLocks.
-      { apply elem_of_dom. apply elem_of_dom in Hpre. rewrite HlocksDom. done. }
-      destruct HLocknameInLocks as [ x  HLocknameInLocks].
-      rewrite HLocknameInLocks in H.
-        by injection H as ->.
-    }
-    { by destruct Hpre as [ [] Hpre]. }
-    iDestruct (big_sepM2_insert_delete _ _ _ unLockArgs false () with "[$Hlockeds $HP]") as "Hlockeds"; eauto.
-    replace (<[unLockArgs:=()]> validLocknames) with (validLocknames).
-    2:{ rewrite insert_id; eauto. by destruct Hpre as [ [] HLocknameValid]. }
-    wp_seq.
-    iApply "Hpost".
-    iSplit; eauto.
+    iDestruct "Hpre" as "[#Hpre HP]".
+    iDestruct (big_sepM_insert_acc with "Hlockeds") as "[_ Hlockeds]"; first done.
+    iSpecialize ("Hlockeds" $! false with "[HP]").
+    { eauto. }
+
+    wp_pures. iApply "Hpost".
+    iSplit; last by eauto.
     iExists _, _; iFrame.
-  }
-  {
-    wp_pures. iApply "Hpost". iSplitL; eauto.
+    replace (dom (gset u64) (<[ln:=false]> locksM)) with (dom (gset u64) locksM); first done.
+    rewrite dom_insert_L.
+    assert (ln ∈ dom (gset u64) locksM).
+    { apply elem_of_dom. eauto. }
+    set_solver.
+  - wp_pures. iApply "Hpost". iSplitL; eauto.
     iExists _, _; iFrame.
-  }
 Qed.
 
-Lemma Clerk__TryLock_spec ck (srv:loc) (ln:u64) γrpc :
+Lemma Clerk__TryLock_spec γ ck (srv:loc) (ln:u64) :
   {{{
-       ⌜is_Some (validLocknames !! ln)⌝
-      ∗ own_clerk ck srv γrpc
-      ∗ is_lockserver srv γrpc 
+    lockservice_is_lock γ ln ∗
+    own_clerk ck srv γ.(ls_rpcGN) ∗
+    is_lockserver srv γ 
   }}}
     Clerk__TryLock ck #ln
-    {{{ v, RET v; ∃(b:u64), ⌜v = #b⌝ ∗ own_clerk ck srv γrpc ∗ (⌜b = 0⌝ ∨ ⌜b = 1⌝ ∗ Ps ln) }}}.
+  {{{ v, RET v; ∃(b:u64), ⌜v = #b⌝ ∗ own_clerk ck srv γ.(ls_rpcGN) ∗ (⌜b = 0⌝ ∨ ⌜b = 1⌝ ∗ Ps ln) }}}.
 Proof using Type*.
-  iIntros (Φ) "Hpre Hpost".
-  iApply (Clerk__from_core LockServer__tryLock_core "LockServer__TryLock" "CallTryLock" "Clerk__TryLock" with "[] [Hpre]").
+  iIntros (Φ) "(#Htok & Hclerk & #[Hinv Hserver]) Hpost".
+  iApply (Clerk__from_core LockServer__tryLock_core "LockServer__TryLock" "CallTryLock" "Clerk__TryLock" _ _ _ _ (TryLock_Pre γ) TryLock_Post with "[] [Hclerk]").
   - by unfold name_neq.
-  - iIntros "* % !#". iApply tryLock_core_spec.
-  - eauto.
+  - iIntros "* % !# [??]". iApply tryLock_core_spec; eauto.
+  - eauto with iFrame.
   - eauto.
 Qed.
 
-Lemma Clerk__Unlock_spec ck (srv:loc) (ln:u64) γrpc :
+Lemma Clerk__Unlock_spec γ ck (srv:loc) (ln:u64) :
   {{{
-       (⌜is_Some (validLocknames !! ln)⌝
-      ∗ Ps ln)
-      ∗ own_clerk ck srv γrpc
-      ∗ is_lockserver srv γrpc 
+    lockservice_is_lock γ ln ∗
+    Ps ln ∗
+    own_clerk ck srv γ.(ls_rpcGN) ∗
+    is_lockserver srv γ 
   }}}
     Clerk__Unlock ck #ln
-    {{{ v, RET v; ∃(b:u64), ⌜v = #b⌝ ∗ own_clerk ck srv γrpc ∗ True }}}.
+    {{{ v, RET v; ∃(b:u64), ⌜v = #b⌝ ∗ own_clerk ck srv γ.(ls_rpcGN) ∗ True }}}.
 Proof using Type*.
-  iIntros (Φ) "Hpre Hpost".
-  iApply (Clerk__from_core LockServer__unlock_core "LockServer__Unlock" "CallUnlock" "Clerk__Unlock" with "[] [Hpre]").
+  iIntros (Φ) "(#Htok & HP & Hclerk & #[Hinv Hserver]) Hpost".
+  iApply (Clerk__from_core LockServer__unlock_core "LockServer__Unlock" "CallUnlock" "Clerk__Unlock" _ _ _ _ (Unlock_Pre γ) Unlock_Post with "[] [Hclerk HP]").
   - by unfold name_neq.
   - iIntros "* % !#". iApply unlock_core_spec.
-  - eauto.
+  - eauto with iFrame.
   - eauto.
 Qed.
 
-Lemma Clerk__Lock_spec ck (srv:loc) (ln:u64) γrpc :
+Lemma Clerk__Lock_spec γ ck (srv:loc) (ln:u64) :
   {{{
-       ⌜is_Some (validLocknames !! ln)⌝
-      ∗ own_clerk ck srv γrpc
-      ∗ is_lockserver srv γrpc
+    lockservice_is_lock γ ln ∗
+    own_clerk ck srv γ.(ls_rpcGN) ∗
+    is_lockserver srv γ
   }}}
     Clerk__Lock ck #ln
-  {{{ RET #true; own_clerk ck srv γrpc ∗ Ps ln }}}.
+  {{{ RET #true; own_clerk ck srv γ.(ls_rpcGN) ∗ Ps ln }}}.
 Proof using Type*.
-  iIntros (Φ) "[% [Hclerk_own #Hinv]] Hpost".
+  iIntros (Φ) "[#Htok [Hclerk_own #Hinv]] Hpost".
   wp_lam.
   wp_pures.
   wp_apply (wp_forBreak
               (fun c =>
-                 (own_clerk ck srv γrpc ∗ Ps ln -∗ Φ #true)
-                 ∗ own_clerk ck srv γrpc
+                 (own_clerk ck srv _ ∗ Ps ln -∗ Φ #true)
+                 ∗ own_clerk ck srv _
                  ∗ (⌜c = true⌝ ∨ ⌜c = false⌝∗ Ps ln)
               )%I
            with "[] [$Hclerk_own $Hpost]"); eauto.
